LeanLgtm/Util.lean
@@ -65,8 +65,15 @@ initialize
 
 abbrev HintExtState := List Syntax
 
+abbrev RevExtState := List Ident
+
+
 initialize hintExt : EnvExtension HintExtState ←
   registerEnvExtension (pure [])
+
+initialize revExt : EnvExtension RevExtState ←
+  registerEnvExtension (pure [])
+
 
 syntax "{|" tacticSeq "|}" : term
 
