LeanLgtm/WP.lean
@@ -1,4 +1,4 @@
-import Ssreflect.Lang
+-- import Ssreflect.Lang
 import Mathlib.Data.Finmap
 import LeanLgtm.Util
 
